src/localdrfra/Stable.v
@@ -469,7 +469,7 @@ Module Stable.
           (NORMAL_MEM1: normal_memory mem1)
           (STABLE_TVIEW1: stable_tview mem1 lc1.(Local.tview))
           (STABLE_MEM1: stable_memory rels mem1)
-          (RELS_WF1: ReleaseWrites.wf rels lc1 mem1)
+          (RELS_WF1: ReleaseWrites.wf rels lc1.(Local.promises) mem1)
           (MSG: forall val released
                   (MSG: msg = Message.concrete val (Some released)),
               normal_view released /\ stable_view mem2 released)
@@ -478,7 +478,7 @@ Module Stable.
       <<NORMAL_MEM2: normal_memory mem2>> /\
       <<STABLE_TVIEW2: stable_tview mem2 lc2.(Local.tview)>> /\
       <<STABLE_MEM2: stable_memory rels mem2>> /\
-      <<RELS_WF2: ReleaseWrites.wf rels lc2 mem2>>.
+      <<RELS_WF2: ReleaseWrites.wf rels lc2.(Local.promises) mem2>>.
     Proof.
       inv STEP. exploit promise; try apply WF1; eauto. i. des.
       splits; auto. ii. ss.
@@ -577,14 +577,14 @@ Module Stable.
           (NORMAL_MEM1: normal_memory mem1)
           (STABLE_TVIEW1: stable_tview mem1 lc1.(Local.tview))
           (STABLE_MEM1: stable_memory rels mem1)
-          (RELS_WF1: ReleaseWrites.wf rels lc1 mem1)
+          (RELS_WF1: ReleaseWrites.wf rels lc1.(Local.promises) mem1)
           (LOC: L loc)
           (REL: List.In (loc, to) rels)
           (ORD: Ordering.le Ordering.acqrel ord)
           (STEP: Local.read_step lc1 mem1 loc to val released ord lc2):
       <<NORMAL_TVIEW2: normal_tview lc2.(Local.tview)>> /\
       <<STABLE_TVIEW2: stable_tview mem1 lc2.(Local.tview)>> /\
-      <<RELS_WF2: ReleaseWrites.wf rels lc2 mem1>>.
+      <<RELS_WF2: ReleaseWrites.wf rels lc2.(Local.promises) mem1>>.
     Proof.
       inv STEP. ss. splits; ss.
       - inv NORMAL_TVIEW1. econs; ss.
@@ -672,12 +672,12 @@ Module Stable.
           (NORMAL_MEM1: normal_memory mem1)
           (STABLE_TVIEW1: stable_tview mem1 lc1.(Local.tview))
           (STABLE_MEM1: stable_memory rels mem1)
-          (RELS_WF1: ReleaseWrites.wf rels lc1 mem1)
+          (RELS_WF1: ReleaseWrites.wf rels lc1.(Local.promises) mem1)
           (LOC: ~ L loc)
           (STEP: Local.read_step lc1 mem1 loc to val released ord lc2):
       <<NORMAL_TVIEW2: normal_tview lc2.(Local.tview)>> /\
       <<STABLE_TVIEW2: stable_tview mem1 lc2.(Local.tview)>> /\
-      <<RELS_WF2: ReleaseWrites.wf rels lc2 mem1>>.
+      <<RELS_WF2: ReleaseWrites.wf rels lc2.(Local.promises) mem1>>.
     Proof.
       inv STEP. ss. splits; ss.
       - inv NORMAL_TVIEW1. econs; ss.
@@ -709,7 +709,7 @@ Module Stable.
           (WF1: Local.wf lc1 mem1)
           (SC1: Memory.closed_timemap sc1 mem1)
           (MEM1: Memory.closed mem1)
-          (RELS_WF1: ReleaseWrites.wf rels lc1 mem1)
+          (RELS_WF1: ReleaseWrites.wf rels lc1.(Local.promises) mem1)
           (NORMAL_TVIEW1: normal_tview lc1.(Local.tview))
           (NORMAL_MEM1: normal_memory mem1)
           (STABLE_TVIEW1: stable_tview mem1 lc1.(Local.tview))
@@ -724,7 +724,8 @@ Module Stable.
       <<NORMAL_MEM2: normal_memory mem2>> /\
       <<STABLE_TVIEW2: stable_tview mem2 lc2.(Local.tview)>> /\
       <<STABLE_MEM2: stable_memory (if Ordering.le Ordering.acqrel ord then (loc, to) :: rels else rels) mem2>> /\
-      <<RELS_WF2: ReleaseWrites.wf (if Ordering.le Ordering.acqrel ord then (loc, to) :: rels else rels) lc2 mem2>>.
+      <<RELS_WF2: ReleaseWrites.wf (if Ordering.le Ordering.acqrel ord then (loc, to) :: rels else rels) 
+                                   lc2.(Local.promises) mem2>>.
     Proof.
       exploit Local.write_step_future; eauto. i. des.
       inv STEP. inv WRITE. ss.
@@ -973,14 +974,15 @@ Module Stable.
           (NORMAL_MEM1: normal_memory mem1)
           (STABLE_TVIEW1: stable_tview mem1 lc1.(Local.tview))
           (STABLE_MEM1: stable_memory rels mem1)
-          (RELS_WF1: ReleaseWrites.wf rels lc1 mem1)
+          (RELS_WF1: ReleaseWrites.wf rels lc1.(Local.promises) mem1)
           (LOC: L loc)
           (STEP: Local.write_step lc1 sc1 mem1 loc from to val None released ord lc2 sc2 mem2 kind):
       <<NORMAL_TVIEW2: normal_tview lc2.(Local.tview)>> /\
       <<NORMAL_MEM2: normal_memory mem2>> /\
       <<STABLE_TVIEW2: stable_tview mem2 lc2.(Local.tview)>> /\
       <<STABLE_MEM2: stable_memory (if Ordering.le Ordering.acqrel ord then (loc, to) :: rels else rels) mem2>> /\
-      <<RELS_WF2: ReleaseWrites.wf (if Ordering.le Ordering.acqrel ord then (loc, to) :: rels else rels) lc2 mem2>>.
+      <<RELS_WF2: ReleaseWrites.wf (if Ordering.le Ordering.acqrel ord then (loc, to) :: rels else rels) 
+                                   lc2.(Local.promises) mem2>>.
     Proof.
       eapply write_step_loc; eauto; ss.
       - apply View.bot_spec.
@@ -995,7 +997,7 @@ Module Stable.
           (NORMAL_MEM1: normal_memory mem1)
           (STABLE_TVIEW1: stable_tview mem1 lc1.(Local.tview))
           (STABLE_MEM1: stable_memory rels mem1)
-          (RELS_WF1: ReleaseWrites.wf rels lc1 mem1)
+          (RELS_WF1: ReleaseWrites.wf rels lc1.(Local.promises) mem1)
           (LOC: ~ L loc)
           (WF_RELEASEDM: View.opt_wf releasedm)
           (CLOSED_RELEASEDM: Memory.closed_opt_view releasedm mem1)
@@ -1006,7 +1008,7 @@ Module Stable.
       <<NORMAL_MEM2: normal_memory mem2>> /\
       <<STABLE_TVIEW2: stable_tview mem2 lc2.(Local.tview)>> /\
       <<STABLE_MEM2: stable_memory rels mem2>> /\
-      <<RELS_WF2: ReleaseWrites.wf rels lc2 mem2>>.
+      <<RELS_WF2: ReleaseWrites.wf rels lc2.(Local.promises) mem2>>.
     Proof.
       exploit Local.write_step_future; eauto. i. des.
       inv STEP. inv WRITE. ss.
@@ -1168,14 +1170,14 @@ Module Stable.
           (NORMAL_MEM1: normal_memory mem1)
           (STABLE_TVIEW1: stable_tview mem1 lc1.(Local.tview))
           (STABLE_MEM1: stable_memory rels mem1)
-          (RELS_WF1: ReleaseWrites.wf rels lc1 mem1)
+          (RELS_WF1: ReleaseWrites.wf rels lc1.(Local.promises) mem1)
           (LOC: ~ L loc)
           (STEP: Local.write_step lc1 sc1 mem1 loc from to val None released ord lc2 sc2 mem2 kind):
       <<NORMAL_TVIEW2: normal_tview lc2.(Local.tview)>> /\
       <<NORMAL_MEM2: normal_memory mem2>> /\
       <<STABLE_TVIEW2: stable_tview mem2 lc2.(Local.tview)>> /\
       <<STABLE_MEM2: stable_memory rels mem2>> /\
-      <<RELS_WF2: ReleaseWrites.wf rels lc2 mem2>>.
+      <<RELS_WF2: ReleaseWrites.wf rels lc2.(Local.promises) mem2>>.
     Proof.
       eapply write_step_other; eauto; ss.
       apply bot_stable_view. apply MEM1.
@@ -1187,12 +1189,12 @@ Module Stable.
           (NORMAL_TVIEW1: normal_tview lc1.(Local.tview))
           (STABLE_TVIEW1: stable_tview mem1 lc1.(Local.tview))
           (STABLE_SC1: stable_timemap mem1 sc1)
-          (RELS_WF1: ReleaseWrites.wf rels lc1 mem1)
+          (RELS_WF1: ReleaseWrites.wf rels lc1.(Local.promises) mem1)
           (STEP: Local.fence_step lc1 sc1 ordr ordw lc2 sc2):
       <<NORMAL_TVIEW2: normal_tview lc2.(Local.tview)>> /\
       <<STABLE_TVIEW2: stable_tview mem1 lc2.(Local.tview)>> /\
       <<STABLE_SC2: stable_timemap mem1 sc2>> /\
-      <<RELS_WF2: ReleaseWrites.wf rels lc2 mem1>>.
+      <<RELS_WF2: ReleaseWrites.wf rels lc2.(Local.promises) mem1>>.
     Proof.
       inv STEP. ss. splits; ss.
       - inv NORMAL_TVIEW1.
